

Readme

1. This Appendix presents the validation process with Laplace's equation for physical components of second- and third-order potential gradients in Tables 3 - 15.
2. In the following parts, the symbol "*" is omitted for simplicity.
3. Each of the following sections is independent by using the command **Clear["Global`*"]** to clear previous arguments.
4. After running all codes, the related results of Laplace's equation in Appendix B are obtained.

Table 3

```
In[*]:= Clear["Global`*"];
```

$$In[*]:= Vrr = \frac{(x^2 * Vxx + 2 * x * y * Vxy + y^2 * Vyy)}{(x^2 + y^2)};$$
$$In[*]:= V\lambda\lambda = \frac{(y^2 * Vxx - 2 * x * y * Vxy + x^2 * Vyy)}{(x^2 + y^2)};$$

```
In[*]:= Vzz = Vzz;
```

$$In[*]:= Vrrr = \frac{(x^3 * Vxxx + 3 * x^2 * y * Vxxy + 3 * x * y^2 * Vyyx + y^3 * Vyyy)}{(x^2 + y^2)^{3/2}};$$
$$In[*]:= Vrr\lambda = \frac{(-x^2 * y * Vxxx + x * (x^2 - 2 * y^2) * Vxxy + y * (2 * x^2 - y^2) * Vyyx + x * y^2 * Vyyy)}{(x^2 + y^2)^{3/2}};$$
$$In[*]:= Vrrz = \frac{(x^2 * Vxxz + 2 * x * y * Vxyz + y^2 * Vyyz)}{(x^2 + y^2)};$$
$$In[*]:= V\lambda\lambda r = \frac{(x * y^2 * Vxxx + y * (y^2 - 2 * x^2) * Vxxy + x * (x^2 - 2 * y^2) * Vyyx + x^2 * y * Vyyy)}{(x^2 + y^2)^{3/2}};$$
$$In[*]:= V\lambda\lambda\lambda = \frac{(-y^3 * Vxxx + 3 * x * y^2 * Vxxy - 3 * x^2 * y * Vyyx + x^3 * Vyyy)}{(x^2 + y^2)^{3/2}};$$
$$In[*]:= V\lambda\lambda z = \frac{(y^2 * Vxxz - 2 * x * y * Vxyz + x^2 * Vyyz)}{(x^2 + y^2)};$$
$$In[*]:= Vzzr = \frac{(x * Vzzx + y * Vzzy)}{\sqrt{x^2 + y^2}};$$
$$In[*]:= Vzz\lambda = \frac{(-y * Vzzx + x * Vzzy)}{\sqrt{x^2 + y^2}};$$

```
In[*]:= Vzzz = Vzzz;
```

```
In[*]:= FullSimplify[Vrr + V\lambda\lambda + Vzz]
```

```
Out[*]=
```

$$Vxx + Vyy + Vzz$$

```
In[*]:= FullSimplify[Vrrr + V\lambda\lambda r + Vzzr]
```

```
Out[*]=
```

$$\frac{(Vxxx + Vyyx + Vzzx) x + (Vxxy + Vyyy + Vzzy) y}{\sqrt{x^2 + y^2}}$$

```
In[*]:= FullSimplify[Vrrλ + Vλλλ + Vzzλ]
Out[*]=
```

$$\frac{(V_{xxy} + V_{yyy} + V_{zzy}) x - (V_{xxx} + V_{yyx} + V_{zzx}) y}{\sqrt{x^2 + y^2}}$$

```
In[*]:= FullSimplify[Vrrz + Vλλz + Vzzz]
Out[*]=
```

$$V_{xxz} + V_{yyz} + V_{zzz}$$

Table 4

```
In[*]:= Clear["Global`*"];

In[*]:= Vrr = (Cos[λ])^2 * Vxx + Sin[2 * λ] * Vxy + (Sin[λ])^2 * Vyy;
In[*]:= Vλλ = (Sin[λ])^2 * Vxx - Sin[2 * λ] * Vxy + (Cos[λ])^2 * Vyy;
In[*]:= Vzz = Vzz;

In[*]:= Vrrr = (Cos[λ])^3 * Vxxx + 3 * Sin[λ] * (Cos[λ])^2 * Vxxy +
3 * Cos[λ] * (Sin[λ])^2 * Vyyx + (Sin[λ])^3 * Vyyy;
In[*]:= Vrrλ = -Sin[λ] * (Cos[λ])^2 * Vxxx + Cos[λ] * ((Cos[λ])^2 - 2 * (Sin[λ])^2) * Vxxy +
Sin[λ] * (2 * (Cos[λ])^2 - (Sin[λ])^2) * Vyyx + (Sin[λ])^2 * Cos[λ] * Vyyy;
In[*]:= Vrrz = (Cos[λ])^2 * Vxxz + Sin[2 * λ] * Vxyz + (Sin[λ])^2 * Vyyz;
In[*]:= Vλλr = Cos[λ] * (Sin[λ])^2 * Vxxx + Sin[λ] * ((Sin[λ])^2 - 2 * (Cos[λ])^2) * Vxxy +
Cos[λ] * ((Cos[λ])^2 - 2 * (Sin[λ])^2) * Vyyx + Sin[λ] * (Cos[λ])^2 * Vyyy;
In[*]:= Vλλλ = - (Sin[λ])^3 * Vxxx + 3 * (Sin[λ])^2 * Cos[λ] * Vxxy -
3 * Sin[λ] * (Cos[λ])^2 * Vyyx + (Cos[λ])^3 * Vyyy;
In[*]:= Vλλz = (Sin[λ])^2 * Vxxz - Sin[2 * λ] * Vxyz + (Cos[λ])^2 * Vyyz;
In[*]:= Vzzr = Cos[λ] * Vzzx + Sin[λ] * Vzzy;
In[*]:= Vzzλ = -Sin[λ] * Vzzx + Cos[λ] * Vzzy;
In[*]:= Vzzz = Vzzz;

In[*]:= FullSimplify[Vrr + Vλλ + Vzz]
Out[*]=
```

$$V_{xx} + V_{yy} + V_{zz}$$

```
In[*]:= FullSimplify[Vrrr + Vλλr + Vzzr]
Out[*]=
```

$$(V_{xxx} + V_{yyx} + V_{zzx}) \cos[\lambda] + (V_{xxy} + V_{yyy} + V_{zzy}) \sin[\lambda]$$

```
In[*]:= FullSimplify[Vrrλ + Vλλλ + Vzzλ]
Out[*]=
```

$$(V_{xxy} + V_{yyy} + V_{zzy}) \cos[\lambda] - (V_{xxx} + V_{yyx} + V_{zzx}) \sin[\lambda]$$

```
In[*]:= FullSimplify[Vrrz + Vλλz + Vzzz]
Out[*]=
```

$$V_{xxz} + V_{yyz} + V_{zzz}$$

Table 5

```

In[*]:= Clear["Global`*"];

In[*]:= Vxx = (x^2 * Vrr - 2 * x * y * Vrl + y^2 * Vll) / (x^2 + y^2);

In[*]:= Vyy = (y^2 * Vrr + 2 * x * y * Vrl + x^2 * Vll) / (x^2 + y^2);

In[*]:= Vzz = Vzz;

In[*]:= Vxxx = (x^3 * Vrrr - 3 * x^2 * y * Vrrl + 3 * x * y^2 * Vllr - y^3 * Vlll) / (x^2 + y^2)^(3/2);

In[*]:= Vxxy =
  (x^2 * y * Vrrr + x * (x^2 - 2 * y^2) * Vrrl + y * (y^2 - 2 * x^2) * Vllr + x * y^2 * Vlll) / (x^2 + y^2)^(3/2);

In[*]:= Vxxz = (x^2 * Vrrz - 2 * x * y * Vrlz + y^2 * Vllz) / (x^2 + y^2);

In[*]:= Vyyx =
  (x * y^2 * Vrrr + y * (2 * x^2 - y^2) * Vrrl + x * (x^2 - 2 * y^2) * Vllr - x^2 * y * Vlll) / (x^2 + y^2)^(3/2);

In[*]:= Vyyy = (y^3 * Vrrr + 3 * x * y^2 * Vrrl + 3 * x^2 * y * Vllr + x^3 * Vlll) / (x^2 + y^2)^(3/2);

In[*]:= Vyyz = (y^2 * Vrrz + 2 * x * y * Vrlz + x^2 * Vllz) / (x^2 + y^2);

In[*]:= Vzzx = (x * Vzzr - y * Vzzl) / Sqrt[x^2 + y^2];

In[*]:= Vzzy = (y * Vzzr + x * Vzzl) / Sqrt[x^2 + y^2];

In[*]:= Vzzz = Vzzz;

In[*]:= FullSimplify[Vxx + Vyy + Vzz]
Out[*]=
  Vrr + Vzz + Vll

In[*]:= FullSimplify[Vxxx + Vyyx + Vzzx]
Out[*]=
  (Vrrr + Vzzr + Vllr) x - (Vrrl + Vzzl + Vlll) y
  / Sqrt[x^2 + y^2]

In[*]:= FullSimplify[Vxxy + Vyyy + Vzzy]
Out[*]=
  (Vrrl + Vzzl + Vlll) x + (Vrrr + Vzzr + Vllr) y
  / Sqrt[x^2 + y^2]

In[*]:= FullSimplify[Vxxz + Vyyz + Vzzz]
Out[*]=
  Vrrz + Vzzz + Vllz

```

Table 6

```

In[*]:= Clear["Global`*"];

In[*]:= Vxx = (Cos[lam])^2 * Vrr - Sin[2 * lam] * Vrl + (Sin[lam])^2 * Vll;

```

```

In[*]:= Vyy = (Sin[λ])2 * Vrr + Sin[2 * λ] * Vrλ + (Cos[λ])2 * Vλλ;
In[*]:= Vzz = Vzz;
In[*]:= Vxxx = (Cos[λ])3 * Vrrr - 3 * Sin[λ] * (Cos[λ])2 * Vrrλ +
          3 * (Sin[λ])2 * Cos[λ] * Vλλr - (Sin[λ])3 * Vλλλ;
In[*]:= Vxxy = Sin[λ] * (Cos[λ])2 * Vrrr + Cos[λ] * ((Cos[λ])2 - 2 * (Sin[λ])2) * Vrrλ +
          Sin[λ] * ((Sin[λ])2 - 2 * (Cos[λ])2) * Vλλr + (Sin[λ])2 * Cos[λ] * Vλλλ;
In[*]:= Vxxz = (Cos[λ])2 * Vrrz - Sin[2 * λ] * Vrλz + (Sin[λ])2 * Vλλz;
In[*]:= Vyyx = (Sin[λ])2 * Cos[λ] * Vrrr + Sin[λ] * (2 * (Cos[λ])2 - (Sin[λ])2) * Vrrλ +
          Cos[λ] * ((Cos[λ])2 - 2 * (Sin[λ])2) * Vλλr - Sin[λ] * (Cos[λ])2 * Vλλλ;
In[*]:= Vyyy = (Sin[λ])3 * Vrrr + 3 * (Sin[λ])2 * Cos[λ] * Vrrλ +
          3 * Sin[λ] * (Cos[λ])2 * Vλλr + (Cos[λ])3 * Vλλλ;
In[*]:= Vyyz = (Sin[λ])2 * Vrrz + Sin[2 * λ] * Vrλz + (Cos[λ])2 * Vλλz;
In[*]:= Vzzx = Cos[λ] * Vzzr - Sin[λ] * Vzzλ;
In[*]:= Vzzy = Sin[λ] * Vzzr + Cos[λ] * Vzzλ;
In[*]:= Vzzz = Vzzz;
In[*]:= FullSimplify[Vxx + Vyy + Vzz]
Out[*]=
      Vrr + Vzz + Vλλ

In[*]:= FullSimplify[Vxxx + Vyyx + Vzzx]
Out[*]=
      (Vrrr + Vzzr + Vλλr) Cos[λ] - (Vrrλ + Vzzλ + Vλλλ) Sin[λ]

In[*]:= FullSimplify[Vxxy + Vyyy + Vzzy]
Out[*]=
      (Vrrλ + Vzzλ + Vλλλ) Cos[λ] + (Vrrr + Vzzr + Vλλr) Sin[λ]

In[*]:= FullSimplify[Vxxz + Vyyz + Vzzz]
Out[*]=
      Vrrz + Vzzz + Vλλz

```

Table 7

```

In[*]:= Clear["Global`*"];
In[*]:= Vλλ = Vλλ;
In[*]:= Vφφ = (z2 * Vrr - 2 * r * z * Vrλ + r2 * Vzz) / (r2 + z2);
In[*]:= Vρρ = (r2 * Vrr + 2 * r * z * Vrλ + z2 * Vzz) / (r2 + z2);
In[*]:= Vλλλ = Vλλλ;
In[*]:= Vλλφ = (-z * Vλλr + r * Vλλz) / √(r2 + z2);
In[*]:= Vλλρ = (r * Vλλr + z * Vλλz) / √(r2 + z2);

```

```

In[*]:= Vφφλ = (z2 * Vrrλ - 2 * r * z * Vrλz + r2 * Vzzλ) / (r2 + z2);

In[*]:= Vφφφ = (-z3 * Vrrr + 3 * r * z2 * Vrrz - 3 * r2 * z * Vzzr + r3 * Vzzz) / (r2 + z2)3/2;

In[*]:= Vφφρ =
  (r * z2 * Vrrr + z * (z2 - 2 * r2) * Vrrz + r * (r2 - 2 * z2) * Vzzr + r2 * z * Vzzz) / (r2 + z2)3/2;

In[*]:= Vρρλ = (r2 * Vrrλ + 2 * r * z * Vrλz + z2 * Vzzλ) / (r2 + z2);

In[*]:= Vρρφ = (-r2 * z * Vrrr + r * (r2 - 2 * z2) * Vrrz + z * (2 * r2 - z2) * Vzzr + r * z2 * Vzzz) /
  (r2 + z2)3/2;

In[*]:= Vρρρ = (r3 * Vrrr + 3 * r2 * z * Vrrz + 3 * r * z2 * Vzzr + z3 * Vzzz) / (r2 + z2)3/2;

In[*]:= FullSimplify[Vλλ + Vφφ + Vρρ]
Out[*]=
  Vrr + Vzz + Vλλ

In[*]:= FullSimplify[Vλλλ + Vφφλ + Vρρλ]
Out[*]=
  Vrrλ + Vzzλ + Vλλλ

In[*]:= FullSimplify[Vλλφ + Vφφφ + Vρρφ]
Out[*]=
  r (Vrrz + Vzzz + Vλλz) - (Vrrr + Vzzr + Vλλr) z
  ───────────────────────────────────
  √(r2 + z2)

In[*]:= FullSimplify[Vλλρ + Vφφρ + Vρρρ]
Out[*]=
  r (Vrrr + Vzzr + Vλλr) + (Vrrz + Vzzz + Vλλz) z
  ───────────────────────────────────
  √(r2 + z2)

```

Table 8

```

In[*]:= Clear["Global`*"];

In[*]:= Vλλ = Vλλ;

In[*]:= Vφφ = (Sin[φ])2 * Vrr - Sin[2 * φ] * Vrλz + (Cos[φ])2 * Vzz;

In[*]:= Vρρ = (Cos[φ])2 * Vrr + Sin[2 * φ] * Vrλz + (Sin[φ])2 * Vzz;

In[*]:= Vλλλ = Vλλλ;

In[*]:= Vλλφ = -Sin[φ] * Vλλr + Cos[φ] * Vλλz;

In[*]:= Vλλρ = Cos[φ] * Vλλr + Sin[φ] * Vλλz;

In[*]:= Vφφλ = (Sin[φ])2 * Vrrλ - Sin[2 * φ] * Vrλz + (Cos[φ])2 * Vzzλ;

In[*]:= Vφφφ = -(Sin[φ])3 * Vrrr + 3 * (Sin[φ])2 * Cos[φ] * Vrrz -
  3 * Sin[φ] * (Cos[φ])2 * Vzzr + (Cos[φ])3 * Vzzz;

In[*]:= Vφφρ = (Sin[φ])2 * Cos[φ] * Vrrr + Sin[φ] * ((Sin[φ])2 - 2 * (Cos[φ])2) * Vrrz +
  Cos[φ] * ((Cos[φ])2 - 2 * (Sin[φ])2) * Vzzr + Sin[φ] * (Cos[φ])2 * Vzzz;

```

```

In[*]:= Vρρλ = (Cos[φ])2 * Vrrλ + Sin[2 * φ] * Vrλz + (Sin[φ])2 * Vzzλ;
In[*]:= Vρρφ = -Sin[φ] * (Cos[φ])2 * Vrrr + Cos[φ] * ((Cos[φ])2 - 2 * (Sin[φ])2) * Vrrz +
      Sin[φ] * (2 * (Cos[φ])2 - (Sin[φ])2) * Vzzr + Cos[φ] * (Sin[φ])2 * Vzzz;
In[*]:= Vρρρ = (Cos[φ])3 * Vrrr + 3 * Sin[φ] * (Cos[φ])2 * Vrrz +
      3 * Cos[φ] * (Sin[φ])2 * Vzzr + (Sin[φ])3 * Vzzz;
In[*]:= FullSimplify[Vλλ + Vφφ + Vρρ]
Out[*]:=
      Vrr + Vzz + Vλλ

In[*]:= FullSimplify[Vλλλ + Vφφλ + Vρρλ]
Out[*]:=
      Vrrλ + Vzzλ + Vλλλ

In[*]:= FullSimplify[Vλλφ + Vφφφ + Vρρφ]
Out[*]:=
      (Vrrz + Vzzz + Vλλz) Cos[φ] - (Vrrr + Vzzr + Vλλr) Sin[φ]

In[*]:= FullSimplify[Vλλρ + Vφφρ + Vρρρ]
Out[*]:=
      (Vrrr + Vzzr + Vλλr) Cos[φ] + (Vrrz + Vzzz + Vλλz) Sin[φ]

```

Table 9

```

In[*]:= Clear["Global`*"];
In[*]:= Vrr = (z2 * Vφφ - 2 * r * z * Vφρ + r2 * Vρρ) / (r2 + z2);
In[*]:= Vλλ = Vλλ;
In[*]:= Vzz = (r2 * Vφφ + 2 * r * z * Vφρ + z2 * Vρρ) / (r2 + z2);
In[*]:= Vrrr = (-z3 * Vφφφ + 3 * r * z2 * Vφφρ - 3 * r2 * z * Vρρφ + r3 * Vρρρ) / (r2 + z2)3/2;
In[*]:= Vrrλ = (-2 * r * z * Vλφρ + z2 * Vφφλ + r2 * Vρρλ) / (r2 + z2);
In[*]:= Vrrz =
      (r * z2 * Vφφφ + z * (z2 - 2 * r2) * Vφφρ + r * (r2 - 2 * z2) * Vρρφ + r2 * z * Vρρρ) / (r2 + z2)3/2;
In[*]:= Vλλr = (-z * Vλλφ + r * Vλλρ) / √(r2 + z2);
In[*]:= Vλλλ = Vλλλ;
In[*]:= Vλλz = (r * Vλλφ + z * Vλλρ) / √(r2 + z2);
In[*]:= Vzzr = (-r2 * z * Vφφφ + r * (r2 - 2 * z2) * Vφφρ + z * (2 * r2 - z2) * Vρρφ + r * z2 * Vρρρ) /
      (r2 + z2)3/2;
In[*]:= Vzzλ = (2 * r * z * Vλφρ + r2 * Vφφλ + z2 * Vρρλ) / (r2 + z2);
In[*]:= Vzzz = (r3 * Vφφφ + 3 * r2 * z * Vφφρ + 3 * r * z2 * Vρρφ + z3 * Vρρρ) / (r2 + z2)3/2;

```

```

In[*]:= FullSimplify[Vrr + Vλλ + Vzz]
Out[*]=
  Vλλ + Vρρ + Vφφ

In[*]:= FullSimplify[Vrrr + Vλλr + Vzzr]
Out[*]=
  r (Vλλρ + Vρρρ + Vφφρ) - (Vλλφ + Vρρφ + Vφφφ) z
  ───────────────────────────
  √r² + z²

In[*]:= FullSimplify[Vrrλ + Vλλλ + Vzzλ]
Out[*]=
  Vλλλ + Vρρλ + Vφφλ

In[*]:= FullSimplify[Vrrz + Vλλz + Vzzz]
Out[*]=
  r (Vλλφ + Vρρφ + Vφφφ) + (Vλλρ + Vρρρ + Vφφρ) z
  ───────────────────────────
  √r² + z²

```

Table 10

```

In[*]:= Clear["Global`*"];

In[*]:= Vrr = (Sin[φ])² * Vφφ - Sin[2 * φ] * Vφρ + (Cos[φ])² * Vρρ;

In[*]:= Vλλ = Vλλ;

In[*]:= Vzz = (Cos[φ])² * Vφφ + Sin[2 * φ] * Vφρ + (Sin[φ])² * Vρρ;

In[*]:= Vrrr = - (Sin[φ])³ * Vφφφ + 3 * (Sin[φ])² * Cos[φ] * Vφφρ -
  3 * Sin[φ] * (Cos[φ])² * Vρρφ + (Cos[φ])³ * Vρρρ;

In[*]:= Vrrλ = (Sin[φ])² * Vφφλ - Sin[2 * φ] * Vλφρ + (Cos[φ])² * Vρρλ;

In[*]:= Vrrz = (Sin[φ])² * Cos[φ] * Vφφφ + Sin[φ] * ((Sin[φ])² - 2 * (Cos[φ])²) * Vφφρ +
  Cos[φ] * ((Cos[φ])² - 2 * (Sin[φ])²) * Vρρφ + Sin[φ] * (Cos[φ])² * Vρρρ;

In[*]:= Vλλr = -Sin[φ] * Vλλφ + Cos[φ] * Vλλρ;

In[*]:= Vλλλ = Vλλλ;

In[*]:= Vλλz = Cos[φ] * Vλλφ + Sin[φ] * Vλλρ;

In[*]:= Vzzr = -Sin[φ] * (Cos[φ])² * Vφφφ + Cos[φ] * ((Cos[φ])² - 2 * (Sin[φ])²) * Vφφρ +
  Sin[φ] * (2 * (Cos[φ])² - (Sin[φ])²) * Vρρφ + (Sin[φ])² * Cos[φ] * Vρρρ;

In[*]:= Vzzλ = Sin[2 * φ] * Vλφρ + (Cos[φ])² * Vφφλ + (Sin[φ])² * Vρρλ;

In[*]:= Vzzz = (Cos[φ])³ * Vφφφ + 3 * Sin[φ] * (Cos[φ])² * Vφφρ +
  3 * (Sin[φ])² * Cos[φ] * Vρρφ + (Sin[φ])³ * Vρρρ;

In[*]:= FullSimplify[Vrr + Vλλ + Vzz]
Out[*]=
  Vλλ + Vρρ + Vφφ

```

In[*]:= FullSimplify[Vrrr + Vλλr + Vzrz]

Out[*]:= $(V\lambda\lambda\rho + V\rho\rho\rho + V\varphi\varphi\rho) \cos[\varphi] - (V\lambda\lambda\varphi + V\rho\rho\varphi + V\varphi\varphi\varphi) \sin[\varphi]$

In[*]:= FullSimplify[Vrrλ + Vλλλ + Vzλλ]

Out[*]:= $V\lambda\lambda\lambda + V\rho\rho\lambda + V\varphi\varphi\lambda$

In[*]:= FullSimplify[Vrrz + Vλλz + Vzλz]

Out[*]:= $(V\lambda\lambda\varphi + V\rho\rho\varphi + V\varphi\varphi\varphi) \cos[\varphi] + (V\lambda\lambda\rho + V\rho\rho\rho + V\varphi\varphi\rho) \sin[\varphi]$

Tables 11 and 12

In[*]:= Clear["Global`*"];

In[*]:=
$$V_{xx} = \frac{\left(y^2 * (x^2 + y^2 + z^2) * V\lambda\lambda + 2 * x * y * z * \sqrt{x^2 + y^2 + z^2} * V\lambda\varphi - \right. \\ \left. 2 * x * y * \sqrt{x^2 + y^2} * \sqrt{x^2 + y^2 + z^2} * V\lambda\rho + x^2 * z^2 * V\varphi\varphi - \right. \\ \left. 2 * x^2 * z * \sqrt{x^2 + y^2} * V\varphi\rho + x^2 * (x^2 + y^2) * V\rho\rho \right) / \left((x^2 + y^2) * (x^2 + y^2 + z^2) \right);$$

In[*]:=
$$V_{yy} = \frac{\left(x^2 * (x^2 + y^2 + z^2) * V\lambda\lambda - 2 * x * y * z * \sqrt{x^2 + y^2 + z^2} * V\lambda\varphi + \right. \\ \left. 2 * x * y * \sqrt{x^2 + y^2} * \sqrt{x^2 + y^2 + z^2} * V\lambda\rho + y^2 * z^2 * V\varphi\varphi - \right. \\ \left. 2 * y^2 * z * \sqrt{x^2 + y^2} * V\varphi\rho + y^2 * (x^2 + y^2) * V\rho\rho \right) / \left((x^2 + y^2) * (x^2 + y^2 + z^2) \right);$$

In[*]:=
$$V_{zz} = \frac{\left((x^2 + y^2) * V\varphi\varphi + 2 * z * \sqrt{x^2 + y^2} * V\varphi\rho + z^2 * V\rho\rho \right) / (x^2 + y^2 + z^2);$$

In[*]:=
$$V_{xxx} = \frac{\left(-y^3 * (x^2 + y^2 + z^2)^{3/2} * V\lambda\lambda\lambda - 3 * x * y^2 * z * (x^2 + y^2 + z^2) * V\lambda\lambda\varphi + 3 * x * y^2 * \sqrt{x^2 + y^2} * \right. \\ \left(x^2 + y^2 + z^2 \right) * V\lambda\lambda\rho + 6 * x^2 * y * z * \sqrt{x^2 + y^2} * \sqrt{x^2 + y^2 + z^2} * V\lambda\varphi\rho - \\ 3 * x^2 * y * z^2 * \sqrt{x^2 + y^2 + z^2} * V\varphi\varphi\lambda - x^3 * z^3 * V\varphi\varphi\varphi + 3 * x^3 * z^2 * \sqrt{x^2 + y^2} * V\varphi\varphi\rho - \\ 3 * x^2 * y * (x^2 + y^2) * \sqrt{x^2 + y^2 + z^2} * V\rho\rho\lambda - 3 * x^3 * z * (x^2 + y^2) * V\rho\rho\varphi + \\ \left. x^3 * (x^2 + y^2)^{3/2} * V\rho\rho\rho \right) / \left((x^2 + y^2)^{3/2} * (x^2 + y^2 + z^2)^{3/2} \right);$$

In[*]:=
$$V_{xxy} = \frac{\left(x * y^2 * (x^2 + y^2 + z^2)^{3/2} * V\lambda\lambda\lambda + y * z * (2 * x^2 - y^2) * (x^2 + y^2 + z^2) * V\lambda\lambda\varphi - \right. \\ y * \sqrt{x^2 + y^2} * (2 * x^2 - y^2) * (x^2 + y^2 + z^2) * V\lambda\lambda\rho - \\ 2 * x * z * (x^2 - 2 * y^2) * \sqrt{x^2 + y^2} * \sqrt{x^2 + y^2 + z^2} * V\lambda\varphi\rho + x * z^2 * (x^2 - 2 * y^2) * \\ \sqrt{x^2 + y^2 + z^2} * V\varphi\varphi\lambda - x^2 * y * z^3 * V\varphi\varphi\varphi + 3 * x^2 * y * z^2 * \sqrt{x^2 + y^2} * V\varphi\varphi\rho + \\ x * (x^4 - x^2 * y^2 - 2 * y^4) * \sqrt{x^2 + y^2 + z^2} * V\rho\rho\lambda - 3 * x^2 * y * z * (x^2 + y^2) * V\rho\rho\varphi + \\ \left. x^2 * y * (x^2 + y^2)^{3/2} * V\rho\rho\rho \right) / \left((x^2 + y^2)^{3/2} * (x^2 + y^2 + z^2)^{3/2} \right);$$

$$In[*]:= Vxxz =$$

$$\begin{aligned} & \left(y^2 * \sqrt{x^2 + y^2} * (x^2 + y^2 + z^2) * V\lambda\lambda\phi + y^2 * z * (x^2 + y^2 + z^2) * V\lambda\lambda\rho - 2 * x * y * (x^2 + y^2 - z^2) * \right. \\ & \quad \sqrt{x^2 + y^2 + z^2} * V\lambda\phi\rho + 2 * x * y * z * \sqrt{x^2 + y^2} * \sqrt{x^2 + y^2 + z^2} * V\phi\phi\lambda + \\ & \quad x^2 * z^2 * \sqrt{x^2 + y^2} * V\phi\phi\phi - x^2 * z * (2 * x^2 + 2 * y^2 - z^2) * V\phi\phi\rho - \\ & \quad 2 * x * y * z * \sqrt{x^2 + y^2} * \sqrt{x^2 + y^2 + z^2} * V\rho\rho\lambda + x^2 * \sqrt{x^2 + y^2} * (x^2 + y^2 - 2 * z^2) * V\rho\rho\phi + \\ & \quad \left. x^2 * z * (x^2 + y^2) * V\rho\rho\rho \right) / \left((x^2 + y^2) * (x^2 + y^2 + z^2)^{3/2} \right); \end{aligned}$$

$$In[*]:= Vyyx = \left(-x^2 * y * (x^2 + y^2 + z^2)^{3/2} * V\lambda\lambda\lambda - x * z * (x^2 - 2 * y^2) * (x^2 + y^2 + z^2) * V\lambda\lambda\phi + \right.$$

$$\begin{aligned} & \quad x * (x^2 - 2 * y^2) * \sqrt{x^2 + y^2} * (x^2 + y^2 + z^2) * V\lambda\lambda\rho - \\ & \quad 2 * y * z * (2 * x^2 - y^2) * \sqrt{x^2 + y^2} * \sqrt{x^2 + y^2 + z^2} * V\lambda\phi\rho + y * z^2 * (2 * x^2 - y^2) * \\ & \quad \sqrt{x^2 + y^2 + z^2} * V\phi\phi\lambda - x * y^2 * z^3 * V\phi\phi\phi + 3 * x * y^2 * z^2 * \sqrt{x^2 + y^2} * V\phi\phi\rho + \\ & \quad y * (2 * x^4 + x^2 * y^2 - y^4) * \sqrt{x^2 + y^2 + z^2} * V\rho\rho\lambda - 3 * x * y^2 * z * (x^2 + y^2) * V\rho\rho\phi + \\ & \quad \left. x * y^2 * (x^2 + y^2)^{3/2} * V\rho\rho\rho \right) / \left((x^2 + y^2)^{3/2} * (x^2 + y^2 + z^2)^{3/2} \right); \end{aligned}$$

$$In[*]:= Vyyy = \left(x^3 * (x^2 + y^2 + z^2)^{3/2} * V\lambda\lambda\lambda - \right.$$

$$\begin{aligned} & \quad 3 * x^2 * y * z * (x^2 + y^2 + z^2) * V\lambda\lambda\phi + 3 * x^2 * y * \sqrt{x^2 + y^2} * (x^2 + y^2 + z^2) * V\lambda\lambda\rho - \\ & \quad 6 * x * y^2 * z * \sqrt{x^2 + y^2} * \sqrt{x^2 + y^2 + z^2} * V\lambda\phi\rho + 3 * x * y^2 * z^2 * \sqrt{x^2 + y^2 + z^2} * V\phi\phi\lambda - \\ & \quad y^3 * z^3 * V\phi\phi\phi + 3 * y^3 * z^2 * \sqrt{x^2 + y^2} * V\phi\phi\rho + 3 * x * y^2 * (x^2 + y^2) * \sqrt{x^2 + y^2 + z^2} * V\rho\rho\lambda - \\ & \quad \left. 3 * y^3 * z * (x^2 + y^2) * V\rho\rho\phi + y^3 * (x^2 + y^2)^{3/2} * V\rho\rho\rho \right) / \left((x^2 + y^2)^{3/2} * (x^2 + y^2 + z^2)^{3/2} \right); \end{aligned}$$

$$In[*]:= Vyyz =$$

$$\begin{aligned} & \left(x^2 * \sqrt{x^2 + y^2} * (x^2 + y^2 + z^2) * V\lambda\lambda\phi + x^2 * z * (x^2 + y^2 + z^2) * V\lambda\lambda\rho + 2 * x * y * (x^2 + y^2 - z^2) * \right. \\ & \quad \sqrt{x^2 + y^2 + z^2} * V\lambda\phi\rho - 2 * x * y * z * \sqrt{x^2 + y^2} * \sqrt{x^2 + y^2 + z^2} * V\phi\phi\lambda + \\ & \quad y^2 * z^2 * \sqrt{x^2 + y^2} * V\phi\phi\phi - y^2 * z * (2 * x^2 + 2 * y^2 - z^2) * V\phi\phi\rho + \\ & \quad 2 * x * y * z * \sqrt{x^2 + y^2} * \sqrt{x^2 + y^2 + z^2} * V\rho\rho\lambda + y^2 * (x^2 + y^2 - 2 * z^2) * \sqrt{x^2 + y^2} * V\rho\rho\phi + \\ & \quad \left. y^2 * z * (x^2 + y^2) * V\rho\rho\rho \right) / \left((x^2 + y^2) * (x^2 + y^2 + z^2)^{3/2} \right); \end{aligned}$$

$$In[*]:= Vzzx = \left(-2 * y * z * \sqrt{x^2 + y^2} * \sqrt{x^2 + y^2 + z^2} * V\lambda\phi\rho - y * (x^2 + y^2) * \sqrt{x^2 + y^2 + z^2} * V\phi\phi\lambda - \right.$$

$$\begin{aligned} & \quad x * z * (x^2 + y^2) * V\phi\phi\phi + x * (x^2 + y^2 - 2 * z^2) * \sqrt{x^2 + y^2} * V\phi\phi\rho - \\ & \quad y * z^2 * \sqrt{x^2 + y^2 + z^2} * V\rho\rho\lambda + x * z * (2 * x^2 + 2 * y^2 - z^2) * V\rho\rho\phi + \\ & \quad \left. x * z^2 * \sqrt{x^2 + y^2} * V\rho\rho\rho \right) / \left(\sqrt{x^2 + y^2} * (x^2 + y^2 + z^2)^{3/2} \right); \end{aligned}$$

$$In[*]:= Vzzy = \left(2 * x * z * \sqrt{x^2 + y^2} * \sqrt{x^2 + y^2 + z^2} * V\lambda\phi\rho + x * (x^2 + y^2) * \sqrt{x^2 + y^2 + z^2} * V\phi\phi\lambda - \right.$$

$$\begin{aligned} & \quad y * z * (x^2 + y^2) * V\phi\phi\phi + y * (x^2 + y^2 - 2 * z^2) * \sqrt{x^2 + y^2} * V\phi\phi\rho + \\ & \quad x * z^2 * \sqrt{x^2 + y^2 + z^2} * V\rho\rho\lambda + y * z * (2 * x^2 + 2 * y^2 - z^2) * V\rho\rho\phi + \\ & \quad \left. y * z^2 * \sqrt{x^2 + y^2} * V\rho\rho\rho \right) / \left(\sqrt{x^2 + y^2} * (x^2 + y^2 + z^2)^{3/2} \right); \end{aligned}$$

$$\text{In[*]:= } \mathbf{Vzzz} = \left((x^2 + y^2)^{3/2} * V\varphi\varphi\varphi + 3 * z * (x^2 + y^2) * V\varphi\varphi\rho + 3 * z^2 * \sqrt{x^2 + y^2} * V\rho\rho\varphi + z^3 * V\rho\rho\rho \right) / (x^2 + y^2 + z^2)^{3/2};$$

In[*]:= FullSimplify[Vxx + Vyy + Vzz]

Out[*]=
 $V\lambda\lambda + V\rho\rho + V\varphi\varphi$

In[*]:= FullSimplify[Vxxx + Vyyx + Vzzx]

Out[*]=

$$\frac{1}{\sqrt{x^2 + y^2} \sqrt{x^2 + y^2 + z^2}} \left((V\lambda\lambda\rho + V\rho\rho\rho + V\varphi\varphi\rho) x \sqrt{x^2 + y^2} - (V\lambda\lambda\varphi + V\rho\rho\varphi + V\varphi\varphi\varphi) x z - (V\lambda\lambda\lambda + V\rho\rho\lambda + V\varphi\varphi\lambda) y \sqrt{x^2 + y^2 + z^2} \right)$$

In[*]:= FullSimplify[Vxxy + Vyyy + Vzzy]

Out[*]=

$$\frac{1}{\sqrt{x^2 + y^2} \sqrt{x^2 + y^2 + z^2}} \left((V\lambda\lambda\rho + V\rho\rho\rho + V\varphi\varphi\rho) y \sqrt{x^2 + y^2} - (V\lambda\lambda\varphi + V\rho\rho\varphi + V\varphi\varphi\varphi) y z + (V\lambda\lambda\lambda + V\rho\rho\lambda + V\varphi\varphi\lambda) x \sqrt{x^2 + y^2 + z^2} \right)$$

In[*]:= FullSimplify[Vxxz + Vyyz + Vzzz]

Out[*]=

$$\frac{(V\lambda\lambda\varphi + V\rho\rho\varphi + V\varphi\varphi\varphi) \sqrt{x^2 + y^2} + (V\lambda\lambda\rho + V\rho\rho\rho + V\varphi\varphi\rho) z}{\sqrt{x^2 + y^2 + z^2}}$$

Table 13

In[*]:= Clear["Global`*"];

In[*]:= $\mathbf{Vxx} = (\text{Sin}[\lambda])^2 * V\lambda\lambda + \text{Sin}[\varphi] * \text{Sin}[2 * \lambda] * V\lambda\varphi - \text{Cos}[\varphi] * \text{Sin}[2 * \lambda] * V\lambda\rho + (\text{Sin}[\varphi])^2 * (\text{Cos}[\lambda])^2 * V\varphi\varphi - \text{Sin}[2 * \varphi] * (\text{Cos}[\lambda])^2 * V\varphi\rho + (\text{Cos}[\varphi])^2 * (\text{Cos}[\lambda])^2 * V\rho\rho;$

In[*]:= $\mathbf{Vyy} = (\text{Cos}[\lambda])^2 * V\lambda\lambda - \text{Sin}[\varphi] * \text{Sin}[2 * \lambda] * V\lambda\varphi + \text{Cos}[\varphi] * \text{Sin}[2 * \lambda] * V\lambda\rho + (\text{Sin}[\varphi])^2 * (\text{Sin}[\lambda])^2 * V\varphi\varphi - \text{Sin}[2 * \varphi] * (\text{Sin}[\lambda])^2 * V\varphi\rho + (\text{Cos}[\varphi])^2 * (\text{Sin}[\lambda])^2 * V\rho\rho;$

In[*]:= $\mathbf{Vzz} = (\text{Cos}[\varphi])^2 * V\varphi\varphi + \text{Sin}[2 * \varphi] * V\varphi\rho + (\text{Sin}[\varphi])^2 * V\rho\rho;$

In[*]:= $\mathbf{Vxxx} = -(\text{Sin}[\lambda])^3 * V\lambda\lambda + 3 * \text{Cos}[\varphi] * (\text{Sin}[\lambda])^2 * \text{Cos}[\lambda] * V\lambda\lambda\rho - 3 * \text{Sin}[\varphi] * (\text{Sin}[\lambda])^2 * \text{Cos}[\lambda] * V\lambda\lambda\varphi + 3 * \text{Sin}[2 * \varphi] * \text{Sin}[\lambda] * (\text{Cos}[\lambda])^2 * V\lambda\varphi\rho - 3 * (\text{Sin}[\varphi])^2 * \text{Sin}[\lambda] * (\text{Cos}[\lambda])^2 * V\varphi\varphi\lambda - (\text{Sin}[\varphi])^3 * (\text{Cos}[\lambda])^3 * V\varphi\varphi\varphi + 3 * (\text{Sin}[\varphi])^2 * \text{Cos}[\varphi] * (\text{Cos}[\lambda])^3 * V\varphi\varphi\rho - 3 * (\text{Cos}[\varphi])^2 * \text{Sin}[\lambda] * (\text{Cos}[\lambda])^2 * V\rho\rho\lambda - 3 * \text{Sin}[\varphi] * (\text{Cos}[\varphi])^2 * (\text{Cos}[\lambda])^3 * V\rho\rho\varphi + (\text{Cos}[\varphi])^3 * (\text{Cos}[\lambda])^3 * V\rho\rho\rho;$

$$\begin{aligned} In[*] := V_{xxy} = & (\sin[\lambda])^2 * \cos[\lambda] * V_{\lambda\lambda\lambda} + \sin[\varphi] * \sin[\lambda] * (2 * (\cos[\lambda])^2 - (\sin[\lambda])^2) * V_{\lambda\lambda\varphi} + \\ & \cos[\varphi] * \sin[\lambda] * ((\sin[\lambda])^2 - 2 * (\cos[\lambda])^2) * V_{\lambda\lambda\rho} + \\ & \sin[2 * \varphi] * \cos[\lambda] * (2 * (\sin[\lambda])^2 - (\cos[\lambda])^2) * V_{\lambda\varphi\rho} + \\ & (\sin[\varphi])^2 * \cos[\lambda] * ((\cos[\lambda])^2 - 2 * (\sin[\lambda])^2) * V_{\varphi\varphi\lambda} - (\sin[\varphi])^3 * \sin[\lambda] * \\ & (\cos[\lambda])^2 * V_{\varphi\varphi\varphi} + 3 * (\sin[\varphi])^2 * \cos[\varphi] * \sin[\lambda] * (\cos[\lambda])^2 * V_{\varphi\varphi\rho} + \\ & (\cos[\varphi])^2 * \cos[\lambda] * ((\cos[\lambda])^2 - 2 * (\sin[\lambda])^2) * V_{\rho\rho\lambda} - 3 * \sin[\varphi] * \\ & (\cos[\varphi])^2 * \sin[\lambda] * (\cos[\lambda])^2 * V_{\rho\rho\varphi} + (\cos[\varphi])^3 * \sin[\lambda] * (\cos[\lambda])^2 * V_{\rho\rho\rho}; \end{aligned}$$

$$\begin{aligned} In[*] := V_{xxz} = & \cos[\varphi] * (\sin[\lambda])^2 * V_{\lambda\lambda\varphi} + \sin[\varphi] * (\sin[\lambda])^2 * V_{\lambda\lambda\rho} - \cos[2 * \varphi] * \sin[2 * \lambda] * V_{\lambda\varphi\rho} + \\ & \sin[\varphi] * \cos[\varphi] * \sin[2 * \lambda] * V_{\varphi\varphi\lambda} + (\sin[\varphi])^2 * \cos[\varphi] * (\cos[\lambda])^2 * V_{\varphi\varphi\varphi} + \\ & \sin[\varphi] * (\cos[\lambda])^2 * ((\sin[\varphi])^2 - 2 * (\cos[\varphi])^2) * V_{\varphi\varphi\rho} - \\ & \sin[2 * \varphi] * \sin[\lambda] * \cos[\lambda] * V_{\rho\rho\lambda} + \cos[\varphi] * (\cos[\lambda])^2 * \\ & ((\cos[\varphi])^2 - 2 * (\sin[\varphi])^2) * V_{\rho\rho\varphi} + \sin[\varphi] * (\cos[\varphi])^2 * (\cos[\lambda])^2 * V_{\rho\rho\rho}; \end{aligned}$$

$$\begin{aligned} In[*] := V_{yyx} = & -\sin[\lambda] * (\cos[\lambda])^2 * V_{\lambda\lambda\lambda} - \sin[\varphi] * \cos[\lambda] * ((\cos[\lambda])^2 - 2 * (\sin[\lambda])^2) * V_{\lambda\lambda\varphi} + \\ & \cos[\varphi] * \cos[\lambda] * ((\cos[\lambda])^2 - 2 * (\sin[\lambda])^2) * V_{\lambda\lambda\rho} - \\ & \sin[2 * \varphi] * \sin[\lambda] * (2 * (\cos[\lambda])^2 - (\sin[\lambda])^2) * V_{\lambda\varphi\rho} + \\ & (\sin[\varphi])^2 * \sin[\lambda] * (2 * (\cos[\lambda])^2 - (\sin[\lambda])^2) * V_{\varphi\varphi\lambda} - (\sin[\varphi])^3 * \\ & (\sin[\lambda])^2 * \cos[\lambda] * V_{\varphi\varphi\varphi} + 3 * (\sin[\varphi])^2 * \cos[\varphi] * (\sin[\lambda])^2 * \cos[\lambda] * V_{\varphi\varphi\rho} + \\ & (\cos[\varphi])^2 * \sin[\lambda] * (2 * (\cos[\lambda])^2 - (\sin[\lambda])^2) * V_{\rho\rho\lambda} - 3 * \sin[\varphi] * \\ & (\cos[\varphi])^2 * (\sin[\lambda])^2 * \cos[\lambda] * V_{\rho\rho\varphi} + (\cos[\varphi])^3 * (\sin[\lambda])^2 * \cos[\lambda] * V_{\rho\rho\rho}; \end{aligned}$$

$$\begin{aligned} In[*] := V_{yyy} = & (\cos[\lambda])^3 * V_{\lambda\lambda\lambda} - 3 * \sin[\varphi] * \sin[\lambda] * (\cos[\lambda])^2 * V_{\lambda\lambda\varphi} + \\ & 3 * \cos[\varphi] * \sin[\lambda] * (\cos[\lambda])^2 * V_{\lambda\lambda\rho} - 3 * \sin[2 * \varphi] * (\sin[\lambda])^2 * \cos[\lambda] * V_{\lambda\varphi\rho} + \\ & 3 * (\sin[\varphi])^2 * (\sin[\lambda])^2 * \cos[\lambda] * V_{\varphi\varphi\lambda} - (\sin[\varphi])^3 * (\sin[\lambda])^3 * V_{\varphi\varphi\varphi} + \\ & 3 * (\sin[\varphi])^2 * \cos[\varphi] * (\sin[\lambda])^3 * V_{\varphi\varphi\rho} + 3 * (\cos[\varphi])^2 * (\sin[\lambda])^2 * \cos[\lambda] * V_{\rho\rho\lambda} - \\ & 3 * \sin[\varphi] * (\cos[\varphi])^2 * (\sin[\lambda])^3 * V_{\rho\rho\varphi} + (\cos[\varphi])^3 * (\sin[\lambda])^3 * V_{\rho\rho\rho}; \end{aligned}$$

$$\begin{aligned} In[*] := V_{yyz} = & \cos[\varphi] * (\cos[\lambda])^2 * V_{\lambda\lambda\varphi} + \sin[\varphi] * (\cos[\lambda])^2 * V_{\lambda\lambda\rho} + \cos[2 * \varphi] * \sin[2 * \lambda] * V_{\lambda\varphi\rho} - \\ & \sin[2 * \varphi] * \sin[\lambda] * \cos[\lambda] * V_{\varphi\varphi\lambda} + (\sin[\varphi])^2 * \cos[\varphi] * (\sin[\lambda])^2 * V_{\varphi\varphi\varphi} + \\ & \sin[\varphi] * (\sin[\lambda])^2 * ((\sin[\varphi])^2 - 2 * (\cos[\varphi])^2) * V_{\varphi\varphi\rho} + \\ & \sin[2 * \varphi] * \sin[\lambda] * \cos[\lambda] * V_{\rho\rho\lambda} + \cos[\varphi] * (\sin[\lambda])^2 * \\ & ((\cos[\varphi])^2 - 2 * (\sin[\varphi])^2) * V_{\rho\rho\varphi} + \sin[\varphi] * (\cos[\varphi])^2 * (\sin[\lambda])^2 * V_{\rho\rho\rho}; \end{aligned}$$

$$\begin{aligned} In[*] := V_{zzx} = & -\sin[2 * \varphi] * \sin[\lambda] * V_{\lambda\varphi\rho} - \\ & (\cos[\varphi])^2 * \sin[\lambda] * V_{\varphi\varphi\lambda} - \sin[\varphi] * (\cos[\varphi])^2 * \cos[\lambda] * V_{\varphi\varphi\varphi} + \\ & \cos[\varphi] * \cos[\lambda] * ((\cos[\varphi])^2 - 2 * (\sin[\varphi])^2) * V_{\varphi\varphi\rho} - (\sin[\varphi])^2 * \sin[\lambda] * V_{\rho\rho\lambda} + \\ & \sin[\varphi] * \cos[\lambda] * (2 * (\cos[\varphi])^2 - (\sin[\varphi])^2) * V_{\rho\rho\varphi} + \\ & (\sin[\varphi])^2 * \cos[\varphi] * \cos[\lambda] * V_{\rho\rho\rho}; \end{aligned}$$

$$\begin{aligned} In[*] := V_{zzy} = & \sin[2 * \varphi] * \cos[\lambda] * V_{\lambda\varphi\rho} + \\ & (\cos[\varphi])^2 * \cos[\lambda] * V_{\varphi\varphi\lambda} - \sin[\varphi] * (\cos[\varphi])^2 * \sin[\lambda] * V_{\varphi\varphi\varphi} + \\ & \cos[\varphi] * \sin[\lambda] * ((\cos[\varphi])^2 - 2 * (\sin[\varphi])^2) * V_{\varphi\varphi\rho} + (\sin[\varphi])^2 * \cos[\lambda] * V_{\rho\rho\lambda} + \\ & \sin[\varphi] * \sin[\lambda] * (2 * (\cos[\varphi])^2 - (\sin[\varphi])^2) * V_{\rho\rho\varphi} + \\ & (\sin[\varphi])^2 * \cos[\varphi] * \sin[\lambda] * V_{\rho\rho\rho}; \end{aligned}$$

```

In[*]:= Vzzz = (Cos[φ])3 * Vφφφ + 3 * Sin[φ] * (Cos[φ])2 * Vφφρ +
          3 * (Sin[φ])2 * Cos[φ] * Vρρφ + (Sin[φ])3 * Vρρρ;

In[*]:= FullSimplify[Vxx + Vyy + Vzz]
Out[*]=
          Vλλλ + Vρρρ + Vφφφ

In[*]:= FullSimplify[Vxxx + Vyyx + Vzzx]
Out[*]=
          - ( (Vλλλ + Vρρλ + Vφφλ) Sin[λ] ) +
          Cos[λ] ( (Vλλρ + Vρρρ + Vφφρ) Cos[φ] - (Vλλφ + Vρρφ + Vφφφ) Sin[φ] )

In[*]:= FullSimplify[Vxxy + Vyyy + Vzzy]
Out[*]=
          (Vλλλ + Vρρλ + Vφφλ) Cos[λ] +
          Sin[λ] ( (Vλλρ + Vρρρ + Vφφρ) Cos[φ] - (Vλλφ + Vρρφ + Vφφφ) Sin[φ] )

In[*]:= FullSimplify[Vxxz + Vyyz + Vzzz]
Out[*]=
          (Vλλφ + Vρρφ + Vφφφ) Cos[φ] + (Vλλρ + Vρρρ + Vφφρ) Sin[φ]

```

Table 14

```

In[*]:= Clear["Global`*"];

In[*]:= Vλλ = (y2 * Vxx - 2 * x * y * Vxy + x2 * Vyy) / (x2 + y2);

In[*]:= Vφφ = (x2 * z2 * Vxx + 2 * x * y * z2 * Vxy - 2 * x * z * (x2 + y2) * Vxz + y2 * z2 * Vyy -
          2 * y * z * (x2 + y2) * Vyz + (x2 + y2)2 * Vzz) / ((x2 + y2) * (x2 + y2 + z2));

In[*]:= Vρρ =
          (x2 * Vxx + 2 * x * y * Vxy + 2 * x * z * Vxz + 2 * y * z * Vyz + y2 * Vyy + z2 * Vzz) / (x2 + y2 + z2);

In[*]:= Vλλλ = (-y3 * Vxxx + 3 * x * y2 * Vxxy - 3 * x2 * y * Vyyx + x3 * Vyyy) / (x2 + y2)3/2;

In[*]:= Vλλφ = (-x * y2 * z * Vxxx + y * z * (2 * x2 - y2) * Vxxy +
          y2 * (x2 + y2) * Vxxz - 2 * x * y * (x2 + y2) * Vxyz + x * z * (2 * y2 - x2) * Vyyx -
          x2 * y * z * Vyyy + x2 * (x2 + y2) * Vyyz) / ((x2 + y2)3/2 * √(x2 + y2 + z2));

In[*]:= Vλλρ = (x * y2 * Vxxx + y * (y2 - 2 * x2) * Vxxy + y2 * z * Vxxz - 2 * x * y * z * Vxyz +
          x * (x2 - 2 * y2) * Vyyx + x2 * y * Vyyy + x2 * z * Vyyz) / ((x2 + y2) * √(x2 + y2 + z2));

In[*]:= Vφφλ = (-x2 * y * z2 * Vxxx + x * z2 * (x2 - 2 * y2) * Vxxy +
          2 * x * y * z * (x2 + y2) * Vxxz - 2 * z * (x4 - y4) * Vxyz +
          y * z2 * (2 * x2 - y2) * Vyyx + x * y2 * z2 * Vyyy - 2 * x * y * z * (x2 + y2) * Vyyz -
          y * (x2 + y2)2 * Vzzx + x * (x2 + y2)2 * Vzzy) / ((x2 + y2)3/2 * (x2 + y2 + z2));

```

```

In[*]:= Vφφφ = (-x^3 * z^3 * Vxxx - 3 * x^2 * y * z^3 * Vxxy + 3 * x^2 * z^2 * (x^2 + y^2) * Vxxz +
6 * x * y * z^2 * (x^2 + y^2) * Vxyz - 3 * x * y^2 * z^3 * Vyyx - y^3 * z^3 * Vyyy +
3 * y^2 * z^2 * (x^2 + y^2) * Vyyz - 3 * x * z * (x^2 + y^2)^2 * Vzzx -
3 * y * z * (x^2 + y^2)^2 * Vzzy + (x^2 + y^2)^3 * Vzzz) / ((x^2 + y^2)^(3/2) * (x^2 + y^2 + z^2)^(3/2));

In[*]:= Vφφρ = (x^3 * z^2 * Vxxx + 3 * x^2 * y * z^2 * Vxxy +
x^2 * z * (z^2 - 2 * x^2 - 2 * y^2) * Vxxz + 2 * x * y * z * (z^2 - 2 * x^2 - 2 * y^2) * Vxyz +
3 * x * y^2 * z^2 * Vyyx + y^3 * z^2 * Vyyy + y^2 * z * (z^2 - 2 * x^2 - 2 * y^2) * Vyyz +
x * (x^2 + y^2) * (x^2 + y^2 - 2 * z^2) * Vzzx + y * (x^2 + y^2) * (x^2 + y^2 - 2 * z^2) * Vzzy +
z * (x^2 + y^2)^2 * Vzzz) / ((x^2 + y^2) * (x^2 + y^2 + z^2)^(3/2));

In[*]:= Vρρλ = (-x^2 * y * Vxxx + x * (x^2 - 2 * y^2) * Vxxy - 2 * x * y * z * Vxxz +
2 * z * (x^2 - y^2) * Vxyz + y * (2 * x^2 - y^2) * Vyyx + x * y^2 * Vyyy +
2 * x * y * z * Vyyz - y * z^2 * Vzzx + x * z^2 * Vzzy) / (sqrt(x^2 + y^2) * (x^2 + y^2 + z^2));

In[*]:= Vρρφ = (-x^3 * z * Vxxx - 3 * x^2 * y * z * Vxxy + x^2 * (x^2 + y^2 - 2 * z^2) * Vxxz +
2 * x * y * (x^2 + y^2 - 2 * z^2) * Vxyz - 3 * x * y^2 * z * Vyyx - y^3 * z * Vyyy +
y^2 * (x^2 + y^2 - 2 * z^2) * Vyyz + x * z * (2 * x^2 + 2 * y^2 - z^2) * Vzzx + y * z *
(2 * x^2 + 2 * y^2 - z^2) * Vzzy + z^2 * (x^2 + y^2) * Vzzz) / (sqrt(x^2 + y^2) * (x^2 + y^2 + z^2)^(3/2));

In[*]:= Vρρρ = (x^3 * Vxxx + 3 * x^2 * y * Vxxy + 3 * x^2 * z * Vxxz +
6 * x * y * z * Vxyz + 3 * x * y^2 * Vyyx + y^3 * Vyyy + 3 * y^2 * z * Vyyz +
3 * x * z^2 * Vzzx + 3 * y * z^2 * Vzzy + z^3 * Vzzz) / (x^2 + y^2 + z^2)^(3/2);

In[*]:= FullSimplify[Vλλ + Vφφ + Vρρ]
Out[*]=
Vxx + Vyy + Vzz

In[*]:= FullSimplify[Vλλλ + Vφφλ + Vρρλ]
Out[*]=
(Vxxy + Vyyy + Vzzy) x - (Vxxx + Vyyx + Vzzx) y
sqrt(x^2 + y^2)

In[*]:= FullSimplify[Vλλφ + Vφφφ + Vρρφ]
Out[*]=
(Vxxz + Vyyz + Vzzz) (x^2 + y^2) - ((Vxxx + Vyyx + Vzzx) x + (Vxxy + Vyyy + Vzzy) y) z
sqrt(x^2 + y^2) sqrt(x^2 + y^2 + z^2)

In[*]:= FullSimplify[Vλλρ + Vφφρ + Vρρρ]
Out[*]=
(Vxxx + Vyyx + Vzzx) x + (Vxxy + Vyyy + Vzzy) y + (Vxxz + Vyyz + Vzzz) z
sqrt(x^2 + y^2 + z^2)

```

Table A15

```
In[*]:= Clear["Global`*"];
```

$$In[*]:= V\lambda\lambda = (\text{Sin}[\lambda])^2 * V_{xx} - \text{Sin}[2 * \lambda] * V_{xy} + (\text{Cos}[\lambda])^2 * V_{yy};$$

$$In[*]:= V\varphi\varphi = (\text{Sin}[\varphi])^2 * (\text{Cos}[\lambda])^2 * V_{xx} + (\text{Sin}[\varphi])^2 * \text{Sin}[2 * \lambda] * V_{xy} - \text{Sin}[2 * \varphi] * \text{Cos}[\lambda] * V_{xz} +$$

$$(\text{Sin}[\varphi])^2 * (\text{Sin}[\lambda])^2 * V_{yy} - \text{Sin}[2 * \varphi] * \text{Sin}[\lambda] * V_{yz} + (\text{Cos}[\varphi])^2 * V_{zz};$$

$$In[*]:= V\rho\rho = (\text{Cos}[\varphi])^2 * (\text{Cos}[\lambda])^2 * V_{xx} + (\text{Cos}[\varphi])^2 * \text{Sin}[2 * \lambda] * V_{xy} + \text{Sin}[2 * \varphi] * \text{Cos}[\lambda] * V_{xz} +$$

$$(\text{Cos}[\varphi])^2 * (\text{Sin}[\lambda])^2 * V_{yy} + \text{Sin}[2 * \varphi] * \text{Sin}[\lambda] * V_{yz} + (\text{Sin}[\varphi])^2 * V_{zz};$$

$$In[*]:= V\lambda\lambda\lambda = -(\text{Sin}[\lambda])^3 * V_{xxx} + 3 * (\text{Sin}[\lambda])^2 * \text{Cos}[\lambda] * V_{xxy} -$$

$$3 * \text{Sin}[\lambda] * (\text{Cos}[\lambda])^2 * V_{yyx} + (\text{Cos}[\lambda])^3 * V_{yyy};$$

$$In[*]:= V\lambda\lambda\varphi = -\text{Sin}[\varphi] * (\text{Sin}[\lambda])^2 * \text{Cos}[\lambda] * V_{xxx} +$$

$$\text{Sin}[\varphi] * \text{Sin}[\lambda] * (2 * (\text{Cos}[\lambda])^2 - (\text{Sin}[\lambda])^2) * V_{xxy} + \text{Cos}[\varphi] * (\text{Sin}[\lambda])^2 * V_{xxz} -$$

$$\text{Cos}[\varphi] * \text{Sin}[2 * \lambda] * V_{xyz} + \text{Sin}[\varphi] * \text{Cos}[\lambda] * (2 * (\text{Sin}[\lambda])^2 - (\text{Cos}[\lambda])^2) * V_{yyx} -$$

$$\text{Sin}[\varphi] * \text{Sin}[\lambda] * (\text{Cos}[\lambda])^2 * V_{yyy} + \text{Cos}[\varphi] * (\text{Cos}[\lambda])^2 * V_{yyz};$$

$$In[*]:= V\lambda\lambda\rho = \text{Cos}[\varphi] * (\text{Sin}[\lambda])^2 * \text{Cos}[\lambda] * V_{xxx} +$$

$$\text{Cos}[\varphi] * \text{Sin}[\lambda] * ((\text{Sin}[\lambda])^2 - 2 * (\text{Cos}[\lambda])^2) * V_{xxy} + \text{Sin}[\varphi] * (\text{Sin}[\lambda])^2 * V_{xxz} -$$

$$\text{Sin}[\varphi] * \text{Sin}[2 * \lambda] * V_{xyz} + \text{Cos}[\varphi] * \text{Cos}[\lambda] * ((\text{Cos}[\lambda])^2 - 2 * (\text{Sin}[\lambda])^2) * V_{yyx} +$$

$$\text{Cos}[\varphi] * \text{Sin}[\lambda] * (\text{Cos}[\lambda])^2 * V_{yyy} + \text{Sin}[\varphi] * (\text{Cos}[\lambda])^2 * V_{yyz};$$

$$In[*]:= V\varphi\varphi\lambda = -(\text{Sin}[\varphi])^2 * \text{Sin}[\lambda] * (\text{Cos}[\lambda])^2 * V_{xxx} +$$

$$(\text{Sin}[\varphi])^2 * \text{Cos}[\lambda] * ((\text{Cos}[\lambda])^2 - 2 * (\text{Sin}[\lambda])^2) * V_{xxy} +$$

$$\text{Sin}[2 * \varphi] * \text{Sin}[\lambda] * \text{Cos}[\lambda] * V_{xxz} - \text{Sin}[2 * \varphi] * \text{Cos}[2 * \lambda] * V_{xyz} +$$

$$(\text{Sin}[\varphi])^2 * \text{Sin}[\lambda] * (2 * (\text{Cos}[\lambda])^2 - (\text{Sin}[\lambda])^2) * V_{yyx} +$$

$$(\text{Sin}[\varphi])^2 * (\text{Sin}[\lambda])^2 * \text{Cos}[\lambda] * V_{yyy} - \text{Sin}[2 * \varphi] * \text{Sin}[\lambda] * \text{Cos}[\lambda] * V_{yyz} -$$

$$(\text{Cos}[\varphi])^2 * \text{Sin}[\lambda] * V_{zzx} + (\text{Cos}[\varphi])^2 * \text{Cos}[\lambda] * V_{zzy};$$

$$In[*]:= V\varphi\varphi\varphi = -(\text{Sin}[\varphi])^3 * (\text{Cos}[\lambda])^3 * V_{xxx} - 3 * (\text{Sin}[\varphi])^3 * \text{Sin}[\lambda] * (\text{Cos}[\lambda])^2 * V_{xxy} +$$

$$3 * (\text{Sin}[\varphi])^2 * \text{Cos}[\varphi] * (\text{Cos}[\lambda])^2 * V_{xxz} + 3 * (\text{Sin}[\varphi])^2 * \text{Cos}[\varphi] * \text{Sin}[2 * \lambda] * V_{xyz} -$$

$$3 * (\text{Sin}[\varphi])^3 * (\text{Sin}[\lambda])^2 * \text{Cos}[\lambda] * V_{yyx} - (\text{Sin}[\varphi])^3 * (\text{Sin}[\lambda])^3 * V_{yyy} +$$

$$3 * (\text{Sin}[\varphi])^2 * \text{Cos}[\varphi] * (\text{Sin}[\lambda])^2 * V_{yyz} - 3 * \text{Sin}[\varphi] * (\text{Cos}[\varphi])^2 * \text{Cos}[\lambda] * V_{zzx} -$$

$$3 * \text{Sin}[\varphi] * (\text{Cos}[\varphi])^2 * \text{Sin}[\lambda] * V_{zzy} + (\text{Cos}[\varphi])^3 * V_{zzz};$$

$$In[*]:= V\varphi\varphi\rho = (\text{Sin}[\varphi])^2 * \text{Cos}[\varphi] * (\text{Cos}[\lambda])^3 * V_{xxx} + 3 * (\text{Sin}[\varphi])^2 * \text{Cos}[\varphi] * \text{Sin}[\lambda] *$$

$$(\text{Cos}[\lambda])^2 * V_{xxy} + \text{Sin}[\varphi] * (\text{Cos}[\lambda])^2 * ((\text{Sin}[\varphi])^2 - 2 * (\text{Cos}[\varphi])^2) * V_{xxz} +$$

$$\text{Sin}[\varphi] * \text{Sin}[2 * \lambda] * ((\text{Sin}[\varphi])^2 - 2 * (\text{Cos}[\varphi])^2) * V_{xyz} + 3 * (\text{Sin}[\varphi])^2 * \text{Cos}[\varphi] * (\text{Sin}[\lambda])^2 * \text{Cos}[\lambda] * V_{yyx} +$$

$$(\text{Sin}[\varphi])^2 * \text{Cos}[\varphi] * (\text{Sin}[\lambda])^3 * V_{yyy} + \text{Sin}[\varphi] * (\text{Sin}[\lambda])^2 * ((\text{Sin}[\varphi])^2 - 2 * (\text{Cos}[\varphi])^2) * V_{yyz} +$$

$$\text{Cos}[\varphi] * \text{Cos}[\lambda] * ((\text{Cos}[\varphi])^2 - 2 * (\text{Sin}[\varphi])^2) * V_{zzx} +$$

$$\text{Cos}[\varphi] * \text{Sin}[\lambda] * ((\text{Cos}[\varphi])^2 - 2 * (\text{Sin}[\varphi])^2) * V_{zzy} + \text{Sin}[\varphi] * (\text{Cos}[\varphi])^2 * V_{zzz};$$

$$In[*]:= V\rho\rho\lambda = -(\text{Cos}[\varphi])^2 * \text{Sin}[\lambda] * (\text{Cos}[\lambda])^2 * V_{xxx} +$$

$$(\text{Cos}[\varphi])^2 * \text{Cos}[\lambda] * ((\text{Cos}[\lambda])^2 - 2 * (\text{Sin}[\lambda])^2) * V_{xxy} -$$

$$\text{Sin}[2 * \varphi] * \text{Sin}[\lambda] * \text{Cos}[\lambda] * V_{xxz} + \text{Sin}[2 * \varphi] * \text{Cos}[2 * \lambda] * V_{xyz} +$$

$$(\text{Cos}[\varphi])^2 * \text{Sin}[\lambda] * (2 * (\text{Cos}[\lambda])^2 - (\text{Sin}[\lambda])^2) * V_{yyx} +$$

$$(\text{Cos}[\varphi])^2 * (\text{Sin}[\lambda])^2 * \text{Cos}[\lambda] * V_{yyy} + \text{Sin}[2 * \varphi] * \text{Sin}[\lambda] * \text{Cos}[\lambda] * V_{yyz} -$$

$$(\text{Sin}[\varphi])^2 * \text{Sin}[\lambda] * V_{zzx} + (\text{Sin}[\varphi])^2 * \text{Cos}[\lambda] * V_{zzy};$$

```

In[*]:= Vρρφ = -Sin[φ] * (Cos[φ])^2 * (Cos[λ])^3 * Vxxx - 3 * Sin[φ] * (Cos[φ])^2 * Sin[λ] *
  (Cos[λ])^2 * Vxxy + Cos[φ] * (Cos[λ])^2 * ((Cos[φ])^2 - 2 * (Sin[φ])^2) * Vxxz +
  Cos[φ] * Sin[2 * λ] * ((Cos[φ])^2 - 2 * (Sin[φ])^2) * Vxyz -
  3 * Sin[φ] * (Cos[φ])^2 * (Sin[λ])^2 * Cos[λ] * Vyyx - Sin[φ] * (Cos[φ])^2 *
  (Sin[λ])^3 * Vyyy + Cos[φ] * (Sin[λ])^2 * ((Cos[φ])^2 - 2 * (Sin[φ])^2) * Vyyz +
  Sin[φ] * Cos[λ] * (2 * (Cos[φ])^2 - (Sin[φ])^2) * Vzzx +
  Sin[φ] * Sin[λ] * (2 * (Cos[φ])^2 - (Sin[φ])^2) * Vzzy + (Sin[φ])^2 * Cos[φ] * Vzzz;

In[*]:= Vρρρ = (Cos[φ])^3 * (Cos[λ])^3 * Vxxx +
  3 * (Cos[φ])^3 * Sin[λ] * (Cos[λ])^2 * Vxxy + 3 * Sin[φ] * (Cos[φ])^2 * (Cos[λ])^2 * Vxxz +
  3 * Sin[2 * φ] * Cos[φ] * Sin[λ] * Cos[λ] * Vxyz +
  3 * (Cos[φ])^3 * (Sin[λ])^2 * Cos[λ] * Vyyx + (Cos[φ])^3 * (Sin[λ])^3 * Vyyy +
  3 * Sin[φ] * (Cos[φ])^2 * (Sin[λ])^2 * Vyyz + 3 * (Sin[φ])^2 * Cos[φ] * Cos[λ] * Vzzx +
  3 * (Sin[φ])^2 * Cos[φ] * Sin[λ] * Vzzy + (Sin[φ])^3 * Vzzz;

In[*]:= FullSimplify[Vλλ + Vφφ + Vρρ]
Out[*]=
  Vxx + Vyy + Vzz

In[*]:= FullSimplify[Vλλλ + Vφφλ + Vρρλ]
Out[*]=
  (Vxxy + Vyyy + Vzzy) Cos[λ] - (Vxxx + Vyyx + Vzzx) Sin[λ]

In[*]:= FullSimplify[Vλλφ + Vφφφ + Vρρφ]
Out[*]=
  (Vxxz + Vyyz + Vzzz) Cos[φ] -
  ((Vxxx + Vyyx + Vzzx) Cos[λ] + (Vxxy + Vyyy + Vzzy) Sin[λ]) Sin[φ]

In[*]:= FullSimplify[Vλλρ + Vφφρ + Vρρρ]
Out[*]=
  (Vxxx + Vyyx + Vzzx) Cos[λ] Cos[φ] +
  (Vxxy + Vyyy + Vzzy) Cos[φ] Sin[λ] + (Vxxz + Vyyz + Vzzz) Sin[φ]

In[*]:= NotebookSave[EvaluationNotebook[]];

```